tutorial/lithium/primitive_laws.v
@@ -1,7 +1,21 @@
 From iris.program_logic Require Export weakestpre.
+From iris.base_logic.lib Require Export gen_heap.
 From iris.proofmode Require Import tactics.
 From iris.program_logic Require Import ectx_lifting.
-From lithium.tutorial Require Export notation.
+From lithium.tutorial Require Export lang notation.
 
-Class tutorialGS (Σ : gFunctors) := {
+Class tutorialGS (Σ : gFunctors) := TutorialGS {
+    tutorial_invGS : invGS Σ;
+    tutorial_gen_heapGS :: gen_heapGS loc val Σ;
 }.
+
+Global Instance tutorial_irisG `{!tutorialGS Σ} : irisGS tutorial_lang Σ := {
+  iris_invGS := tutorial_invGS;
+  state_interp σ κs _ _ := gen_heap_interp σ.(heap);
+  fork_post _ := True%I;
+  num_laters_per_step _ := 0%nat;
+  state_interp_mono _ _ _ _ := fupd_intro _ _;
+}.
+
+Notation "l ↦ dq v" := (mapsto l dq v)
+  (at level 20, dq custom dfrac at level 1, format "l  ↦ dq  v") : bi_scope.
