tutorial/lithium/tutorial.v
@@ -4,7 +4,7 @@ From lithium Require Import all.
 From lithium.tutorial Require Import lang notation primitive_laws.
 Set Default Proof Using "Type".
 
-(** * Definitions and step *)
+(** * Definitions and setup *)
 Section definitions.
   Context `{!tutorialGS Σ}.
 
@@ -18,6 +18,11 @@ Section definitions.
   Class CheckBinop (op : bin_op) (v1 v2 : val) : Type :=
     check_binop_proof G : iProp_to_Prop (check_binop op v1 v2 G).
 
+  Definition check_unop (op : un_op) (v : val) (G : val → iProp Σ) : iProp Σ.
+  Admitted.
+  Class CheckUnop (op : un_op) (v : val) : Type :=
+    check_unop_proof G : iProp_to_Prop (check_unop op v G).
+
   Definition check_if (v : val) (G1 G2 : iProp Σ) : iProp Σ.
   Admitted.
   Class CheckIf (v : val) : Type :=
@@ -28,6 +33,7 @@ Ltac generate_i2p_instance_to_tc_hook arg c ::=
   lazymatch c with
   | check_expr ?x1 => constr:(CheckExpr x1)
   | check_binop ?x1 ?x2 ?x3 => constr:(CheckBinop x1 x2 x3)
+  | check_unop ?x1 ?x2 => constr:(CheckUnop x1 x2)
   | check_if ?x1 => constr:(CheckIf x1)
   end.
 Ltac liExtensible_to_i2p_hook P bind cont ::=
@@ -36,13 +42,16 @@ Ltac liExtensible_to_i2p_hook P bind cont ::=
       cont uconstr:(((_ : CheckExpr _) _))
   | check_binop ?op ?v1 ?v2 ?G =>
       cont uconstr:(((_ : CheckBinop _ _ _) _))
+  | check_unop ?op ?v ?G =>
+      cont uconstr:(((_ : CheckUnop _ _) _))
   | check_if ?v ?G1 ?G2 =>
       cont uconstr:(((_ : CheckIf _) _ _))
   end.
 
 Ltac liToSyntax_hook ::=
   change (check_expr ?x1) with (li.bind1 (check_expr x1));
-  change (check_binop ?x1 ?x2 ?x3) with (li.bind1 (check_binop x1 x2 x3)).
+  change (check_binop ?x1 ?x2 ?x3) with (li.bind1 (check_binop x1 x2 x3));
+  change (check_unop ?x1 ?x2) with (li.bind1 (check_unop x1 x2)).
 
 Ltac liTStep :=
  liEnsureInvariant;
@@ -268,6 +277,18 @@ Section proofs.
   Definition check_expr_if_inst := [instance check_expr_if].
   Global Existing Instance check_expr_if_inst.
 
+  Lemma check_if_0 G1 G2 :
+    check_if #0 G1 G2 ::= return G2.
+  Proof. Admitted.
+  Definition check_if_0_inst := [instance check_if_0].
+  Global Existing Instance check_if_0_inst | 2.
+
+  Lemma check_if_1 G1 G2 :
+    check_if #1 G1 G2 ::= return G1.
+  Proof. Admitted.
+  Definition check_if_1_inst := [instance check_if_1].
+  Global Existing Instance check_if_1_inst | 2.
+
   Lemma check_if_bool (b : bool) G1 G2 :
     check_if #b G1 G2 ::=
       and:
@@ -275,7 +296,7 @@ Section proofs.
       | inhale ⌜¬ b⌝; return G2.
   Proof. Admitted.
   Definition check_if_bool_inst := [instance check_if_bool].
-  Global Existing Instance check_if_bool_inst | 2.
+  Global Existing Instance check_if_bool_inst | 10.
 
   Lemma fib_correct :
     ⊢ fn_spec fib_code unit (λ _ v, ∃ n : Z, ⌜v = #n⌝ ∗ ⌜0 ≤ n⌝)
@@ -285,9 +306,13 @@ Section proofs.
     repeat liTStep; liShow.
   Abort.
 
+  Global Instance fn_spec_pers X v pre post :
+    Persistent (fn_spec v X pre post).
+  Proof. Admitted.
+
   Global Instance fn_spec_intro_pers X v pre post :
     IntroPersistent (fn_spec v X pre post) (fn_spec v X pre post).
-  Proof. Admitted.
+  Proof. constructor. by iIntros "#?". Qed.
 
   Lemma fib_correct :
     ⊢ fn_spec fib_code unit (λ _ v, ∃ n : Z, ⌜v = #n⌝ ∗ ⌜0 ≤ n⌝)
@@ -302,26 +327,334 @@ Section proofs.
   Qed.
 
   (** * linked lists *)
+  (** ** constructing linked lists *)
   Definition empty_code : val := λ: <>, #NULL.
-  Definition is_empty_code : val := λ: "v", "v" = #NULL.
-  Definition cons_code : val := λ: "l" "v",
-      let: "new_l" := Alloc #2 in
-      "new_l" + #0 <- "v";;
-      "new_l" + #1 <- "l";;
+  Definition cons_code : val := λ: "a",
+      let: "l" := Fst "a" in
+      let: "v" := Snd "a" in
+      let: "new_l" := Alloc in
+      "new_l" <- ("l", "v");;
       "new_l".
-  Definition head_code : val := λ: "l", ! ("l" + #0).
-  Definition tail_code : val := λ: "l",
-      if: "l" = #NULL then #NULL else ! ("l" + #1).
+
+  Definition build_list_code (empty cons : val) : val := λ: <>,
+    let: "l" := empty #0 in
+    let: "l" := cons ("l", #1) in
+    let: "l" := cons ("l", #2) in
+    "l".
+
+  Fixpoint is_list (v : val) (xs : list val) : iProp Σ :=
+    match xs with
+    | [] => ⌜v = #NULL⌝
+    | x :: xs => ∃ (l : loc) vnext, ⌜v = #l⌝ ∗ l ↦ (vnext, x)%V ∗ is_list vnext xs
+  end.
+  Global Typeclasses Opaque is_list.
+  Global Opaque is_list.
+
+  Lemma empty_correct :
+    ⊢ fn_spec empty_code unit (λ _ _, True) (λ _ v, is_list v []).
+  Proof.
+    iStartProof. iApply prove_fn_spec_rec. simpl.
+    repeat liTStep; liShow.
+  Abort.
+
+  Lemma simplify_goal_is_list_null xs G :
+    simplify_goal (is_list #NULL xs) G ::= exhale ⌜xs = []⌝; return G.
+  Proof. Admitted.
+  Definition simplify_goal_is_list_null_inst := [instance simplify_goal_is_list_null with 50%N].
+  Global Existing Instance simplify_goal_is_list_null_inst.
+
+  Lemma empty_correct :
+    ⊢ fn_spec empty_code unit (λ _ _, True) (λ _ v, is_list v []).
+  Proof.
+    iStartProof. iApply prove_fn_spec_rec. simpl.
+    repeat liTStep; liShow.
+  Qed.
+
+
+  Lemma cons_correct :
+    ⊢ fn_spec cons_code (val * list val)
+      (λ '(x, xs) a, ∃ v, ⌜a = (v, x)%V⌝ ∗ is_list v xs)
+      (λ '(x, xs) r, is_list r (x :: xs)).
+  Proof.
+    iStartProof. iApply prove_fn_spec_rec. simpl.
+    repeat liTStep; liShow.
+  Abort.
+
+  Lemma check_expr_unop op e G :
+    check_expr (UnOp op e) G ::=
+      v ← {check_expr e};
+      vr  ← {check_unop op v};
+      return G vr.
+  Proof. Admitted.
+  Definition check_expr_unop_inst := [instance check_expr_unop].
+  Global Existing Instance check_expr_unop_inst.
+
+  Lemma check_unop_fst v1 v2 G :
+    check_unop FstOp (v1, v2) G ::= return G v1.
+  Proof. Admitted.
+  Definition check_unop_fst_inst := [instance check_unop_fst].
+  Global Existing Instance check_unop_fst_inst.
+  Lemma check_unop_snd v1 v2 G :
+    check_unop SndOp (v1, v2) G ::= return G v2.
+  Proof. Admitted.
+  Definition check_unop_snd_inst := [instance check_unop_snd].
+  Global Existing Instance check_unop_snd_inst.
+
+  Lemma check_binop_pair v1 v2 G :
+    check_binop PairOp v1 v2 G ::= return G (v1, v2)%V.
+  Proof. Admitted.
+  Definition check_binop_pair_inst := [instance check_binop_pair].
+  Global Existing Instance check_binop_pair_inst.
+
+  Lemma check_expr_alloc G :
+    check_expr Alloc G ::=
+      ∀ l : loc,
+      inhale (l ↦ #0);
+      return G #l.
+  Proof. Admitted.
+  Definition check_expr_alloc_inst := [instance check_expr_alloc].
+  Global Existing Instance check_expr_alloc_inst.
+
+  Lemma cons_correct :
+    ⊢ fn_spec cons_code (val * list val)
+      (λ '(x, xs) a, ∃ v, ⌜a = (v, x)%V⌝ ∗ is_list v xs)
+      (λ '(x, xs) r, is_list r (x :: xs)).
+  Proof.
+    iStartProof. iApply prove_fn_spec_rec. simpl.
+    repeat liTStep; liShow.
+  Abort.
+
+  Definition FindMapsTo (v : val) :=
+  {| fic_A := (loc * val); fic_Prop '(l, vr) := (⌜v = #l⌝ ∗ l ↦ vr)%I; |}.
+  Global Typeclasses Opaque FindMapsTo.
+
+  Lemma check_expr_store e1 e2 G :
+    check_expr (Store e1 e2) G ::=
+      v2 ← {check_expr e2};
+      v1 ← {check_expr e1};
+      '(l, _) ← {find_in_context (FindMapsTo v1)};
+      inhale (l ↦ v2);
+      return G v2.
+  Proof. Admitted.
+  Definition check_expr_store_inst := [instance check_expr_store].
+  Global Existing Instance check_expr_store_inst.
+
+  Lemma check_expr_load e G :
+    check_expr (Load e) G ::=
+      v ← {check_expr e};
+      '(l, vl) ← {find_in_context (FindMapsTo v)};
+      inhale (l ↦ vl);
+      return G vl.
+  Proof. Admitted.
+  Definition check_expr_load_inst := [instance check_expr_load].
+  Global Existing Instance check_expr_load_inst.
+
+  Lemma cons_correct :
+    ⊢ fn_spec cons_code (val * list val)
+      (λ '(x, xs) a, ∃ v, ⌜a = (v, x)%V⌝ ∗ is_list v xs)
+      (λ '(x, xs) r, is_list r (x :: xs)).
+  Proof.
+    iStartProof. iApply prove_fn_spec_rec. simpl.
+    repeat liTStep; liShow.
+  Abort.
+
+  Lemma find_in_context_find_mapsto_loc (l : loc) G:
+    find_in_context (FindMapsTo #l) G ::=
+      ∃ v,
+      exhale (l ↦ v);
+      return G (l, v).
+  Proof. iDestruct 1 as (v) "[Hl HT]". iExists (_, _) => /=. by iFrame. Qed.
+  Definition find_in_context_find_mapsto_loc_inst :=
+    [instance find_in_context_find_mapsto_loc with FICSyntactic].
+  Global Existing Instance find_in_context_find_mapsto_loc_inst | 1.
+
+  Lemma cons_correct :
+    ⊢ fn_spec cons_code (val * list val)
+      (λ '(x, xs) a, ∃ v, ⌜a = (v, x)%V⌝ ∗ is_list v xs)
+      (λ '(x, xs) r, is_list r (x :: xs)).
+  Proof.
+    iStartProof. iApply prove_fn_spec_rec. simpl.
+    repeat liTStep; liShow.
+  Abort.
+
+  Definition FindList (v : val) :=
+  {| fic_A := iProp Σ; fic_Prop P := P; |}.
+  Global Typeclasses Opaque FindList.
+  Lemma find_in_context_find_list_loc (l : loc) G:
+    find_in_context (FindList #l) G ::=
+      ∃ v, exhale l ↦ v; return G (l ↦ v).
+  Proof. iDestruct 1 as (v) "[Hl HT]". iExists _. by iFrame. Qed.
+  Definition find_in_context_find_list_loc_inst :=
+    [instance find_in_context_find_list_loc with FICSyntactic].
+  Global Existing Instance find_in_context_find_list_loc_inst | 10.
+
+  Global Instance related_to_list v xs : RelatedTo (is_list v xs) | 100 := {| rt_fic := FindList v |}.
+
+  Lemma cons_correct :
+    ⊢ fn_spec cons_code (val * list val)
+      (λ '(x, xs) a, ∃ v, ⌜a = (v, x)%V⌝ ∗ is_list v xs)
+      (λ '(x, xs) r, is_list r (x :: xs)).
+  Proof.
+    iStartProof. iApply prove_fn_spec_rec. simpl.
+    repeat liTStep; liShow.
+  Abort.
+
+  Lemma subsume_mapsto_list (l : loc) v xs G :
+    subsume (l ↦ v) (is_list #l xs) G ::=
+     ∃ v1 v2 xs',
+     exhale ⌜v = (v1, v2)%V⌝ ∗ ⌜xs = v2 :: xs'⌝ ∗ is_list v1 xs';
+     return G.
+  Proof. Admitted.
+  Definition subsume_mapsto_list_inst := [instance subsume_mapsto_list].
+  Global Existing Instance subsume_mapsto_list_inst.
+
+  Lemma cons_correct :
+    ⊢ fn_spec cons_code (val * list val)
+      (λ '(x, xs) a, ∃ v, ⌜a = (v, x)%V⌝ ∗ is_list v xs)
+      (λ '(x, xs) r, is_list r (x :: xs)).
+  Proof.
+    iStartProof. iApply prove_fn_spec_rec. simpl.
+    repeat liTStep; liShow.
+  Qed.
+
+  Lemma build_list_correct empty cons :
+    fn_spec empty unit (λ _ _, True) (λ _ v, is_list v []) -∗
+    fn_spec cons (val * list val) (λ '(x, xs) a, ∃ v, ⌜a = (v, x)%V⌝ ∗ is_list v xs) (λ '(x, xs) r, is_list r (x :: xs)) -∗
+    fn_spec (build_list_code empty cons) unit (λ _ _, True) (λ _ v, is_list v [ #1; #2 ]).
+  Proof.
+    iStartProof. iIntros "#? #?". iApply prove_fn_spec_rec. simpl.
+    repeat liTStep; liShow.
+  Abort.
+
+  Lemma find_in_context_find_list_list v G:
+    find_in_context (FindList v) G ::=
+      ∃ xs, exhale is_list v xs; return G (is_list v xs).
+  Proof. iDestruct 1 as (xs) "[Hl HT]". iExists _. by iFrame. Qed.
+  Definition find_in_context_find_list_list_inst :=
+    [instance find_in_context_find_list_list with FICSyntactic].
+  Global Existing Instance find_in_context_find_list_list_inst | 1.
+
+  Lemma subsume_list_list v xs1 xs2 G :
+    subsume (is_list v xs1) (is_list v xs2) G ::=
+     exhale ⌜xs1 = xs2⌝;
+     return G.
+  Proof. Admitted.
+  Definition subsume_list_list_inst := [instance subsume_list_list].
+  Global Existing Instance subsume_list_list_inst.
+
+
+  Lemma build_list_correct empty cons :
+    fn_spec empty unit (λ _ _, True) (λ _ v, is_list v []) -∗
+    fn_spec cons (val * list val) (λ '(x, xs) a, ∃ v, ⌜a = (v, x)%V⌝ ∗ is_list v xs) (λ '(x, xs) r, is_list r (x :: xs)) -∗
+    fn_spec (build_list_code empty cons) unit (λ _ _, True) (λ _ v, is_list v [ #2; #1 ]).
+  Proof.
+    iStartProof. iIntros "#? #?". iApply prove_fn_spec_rec. simpl.
+    repeat liTStep; liShow.
+  Qed.
+
+  (** ** destructing linked lists *)
+  Definition head_code : val := λ: "l", Snd (! "l").
+
+  Lemma head_correct :
+    ⊢ fn_spec head_code (val * list val)
+      (λ '(va, xs) v, ⌜v = va⌝ ∗ is_list v xs ∗ ⌜0 < length xs⌝)
+      (λ '(va, xs) r, ⌜∃ xs', xs = r::xs'⌝ ∗ is_list va xs).
+  Proof.
+    iStartProof. iApply prove_fn_spec_rec. simpl.
+    repeat liTStep; liShow.
+  Abort.
+
+  Lemma find_in_context_find_mapsto_list v G:
+    find_in_context (FindMapsTo v) G ::=
+      ∃ xs, exhale is_list v xs;
+      exhale ⌜0 < length xs⌝;
+      ∀ (l : loc) v' x xs',
+      inhale ⌜v = #l⌝ ∗ ⌜xs = x::xs'⌝ ∗ is_list v' xs';
+      return G (l, (v', x)%V).
+  Proof. Admitted.
+  Definition find_in_context_find_mapsto_list_inst :=
+    [instance find_in_context_find_mapsto_list with FICSyntactic].
+  Global Existing Instance find_in_context_find_mapsto_list_inst | 10.
+
+  Lemma head_correct :
+    ⊢ fn_spec head_code (val * list val)
+      (λ '(va, xs) v, ⌜v = va⌝ ∗ is_list v xs ∗ ⌜0 < length xs⌝)
+      (λ '(va, xs) r, ⌜∃ xs', xs = r::xs'⌝ ∗ is_list va xs).
+  Proof.
+    iStartProof. iApply prove_fn_spec_rec. simpl.
+    repeat liTStep; liShow.
+    Unshelve. all: unshelve_sidecond.
+    - naive_solver.
+  Qed.
+
+
+
   Definition length_code : val := rec: "f" "l" :=
       if: "l" = #NULL then
         #0
       else
-        let: "r" := "f" (! ("l" + #1)) in
+        let: "r" := "f" (Fst (! "l")) in
         "r" + #1.
-  Definition app_code : val := rec: "f" "x" "y" :=
-      if: !"x" = #NULL then
-        "x" <- "y"
-      else
-        "f" ((! "x") + #1) "y".
+
+  Lemma length_correct :
+    ⊢ fn_spec length_code (val * list val)
+      (λ '(va, xs) v, ⌜v = va⌝ ∗ is_list v xs)
+      (λ '(va, xs) r, ⌜r = #(length xs)⌝ ∗ is_list va xs).
+  Proof.
+    iStartProof. iApply prove_fn_spec_rec. simpl.
+    repeat liTStep; liShow.
+  Abort.
+
+  (* TODO: mention that there are also other approaches to handle this
+  overloading, see RefinedC and Islaris *)
+  Definition FindLocOrNULL (v : val) :=
+  {| fic_A := option loc; fic_Prop o :=
+      match o with | Some l => ⌜v = #l⌝ | None => ⌜v = #NULL⌝ end%I : iProp Σ; |}.
+  Global Typeclasses Opaque FindLocOrNULL.
+
+  Lemma check_binop_eq_val_NULL v G :
+    check_binop EqOp v #NULL G ::=
+      o ← {find_in_context (FindLocOrNULL v)};
+      return G #(if o is Some _ then false else true).
+  Proof. Admitted.
+  Definition check_binop_eq_val_NULL_inst := [instance check_binop_eq_val_NULL].
+  Global Existing Instance check_binop_eq_val_NULL_inst.
+
+  Lemma length_correct :
+    ⊢ fn_spec length_code (val * list val)
+      (λ '(va, xs) v, ⌜v = va⌝ ∗ is_list v xs)
+      (λ '(va, xs) r, ⌜r = #(length xs)⌝ ∗ is_list va xs).
+  Proof.
+    iStartProof. iApply prove_fn_spec_rec. simpl.
+    repeat liTStep; liShow.
+  Abort.
+
+  Lemma find_in_context_find_locornull_list v G:
+    find_in_context (FindLocOrNULL v) G ::=
+      ∃ xs, exhale is_list v xs;
+      and:
+      | inhale ⌜xs = []⌝ ∗ ⌜v = #NULL⌝; return G None
+      | ∀ (l : loc) v' x xs',
+        inhale ⌜v = #l⌝ ∗ ⌜xs = x::xs'⌝ ∗ l ↦ (v', x)%V ∗ is_list v' xs';
+        return G (Some l).
+  Proof. Admitted.
+  Definition find_in_context_find_locornull_list_inst :=
+    [instance find_in_context_find_locornull_list with FICSyntactic].
+  Global Existing Instance find_in_context_find_locornull_list_inst | 10.
+
+  Lemma length_correct :
+    ⊢ fn_spec length_code (val * list val)
+      (λ '(va, xs) v, ⌜v = va⌝ ∗ is_list v xs)
+      (λ '(va, xs) r, ⌜r = #(length xs)⌝ ∗ is_list va xs).
+  Proof.
+    iStartProof. iApply prove_fn_spec_rec. simpl.
+    repeat liTStep; liShow.
+    Unshelve. all: unshelve_sidecond.
+    - do 2 f_equal. lia.
+  Qed.
+
+  (* TODOs:
+     - explain evars somehow
+ *)
 
 End proofs.
